Proof of composability of executions

il2Script.sml
@@ -77,4 +77,75 @@ val (exec_one_rules, exec_one_ind, exec_one_cases) = Hol_reln `
 
 val exec_def = Define `exec P c c' = (exec_one P)^* c c'`;
 
+val exec_strongind = store_thm("exec_strongind",
+``!PR P.
+     (∀x. P x x) ∧ (∀x y z. (exec_one PR) x y ∧ (exec_one PR)^* y z ∧ P y z ⇒ P x z) ⇒
+     !c1 c2. (exec_one PR)^* c1 c2 ⇒ P c1 c2``,
+metis_tac [RTC_STRONG_INDUCT]);
+
+val exec_strongind_right = store_thm("exec_strongind_right",
+``∀R P.
+           (∀x. P x x) ∧ (∀x y z. P x y ∧ (exec_one R)^* x y ∧ (exec_one R) y z ⇒ P x z) ⇒
+           ∀x y. (exec_one R)^* x y ⇒ P x y``,
+metis_tac [RTC_STRONG_INDUCT_RIGHT1]);
+
+
+val APPEND_TRACE_SAME_THM = store_thm("APPEND_TRACE_SAME_THM",
+``!P c c'.exec P c c' ==> !P'.exec (P ++ P') c c'``,
+fs [exec_def] THEN strip_tac THEN ho_match_mp_tac exec_strongind_right THEN rw []
+THEN fs [Once exec_one_cases]
+
+THEN `(exec_one (P ++ P'))^* c (pc, stk, st)` by metis_tac []
+THEN `exec_instr ((P ++ P') !! pc) (pc, stk, st) (pc', stk', st')` by metis_tac [fetch_append_thm, int_ge]
+THEN `(exec_one (P ++ P')) (pc, stk, st) (pc', stk', st')` by rwa [exec_one_cases]
+THEN rw [Once RTC_CASES2] THEN metis_tac []);
+
+val incr_pc_def = Define `incr_pc (i, s, stk) (i':int) = (i + i', s, stk)`;
+
+val CHANGE_PC_INSTR_THM = store_thm("CHANGE_PC_INSTR_THM",
+``!n x pc s stk pc' s' stk'.exec_instr x (pc, s, stk) (pc', s', stk') <=> exec_instr x (n + pc, s, stk) (n + pc', s', stk')``,
+Cases_on `x` THEN rwa [EQ_IMP_THM, exec_instr_cases] THEN Cases_on `s` THEN fsa [exec_instr_cases] THEN rw[] THEN rwa []);
+
+val APPEND_TRACE_SAME_2_THM = store_thm("APPEND_TRACE_SAME_2_THM",
+``!P c c'.exec P c c' ==> !P'.exec (P' ++ P) (incr_pc c (&LENGTH P')) (incr_pc c' (&LENGTH P'))``,
+fs [exec_def] THEN strip_tac
+THEN ho_match_mp_tac exec_strongind_right THEN rw [] THEN Cases_on `c` THEN Cases_on `c'` THEN Cases_on `c''` THEN fs [Once exec_one_cases] THEN rw [] THEN fs [incr_pc_def] THEN rw []
+
+
+THEN `exec_instr ((P' ++ P) !! (q' + &LENGTH P')) (&LENGTH P' + q', stk, st) (&LENGTH P' + q'', stk', st')` by (
+
+`P' ++ P !! q' + &LENGTH P' = P !! q'` by (
+
+`0 <= q' + &LENGTH P'` by fsa [int_ge]
+THEN fsa [fetch_append_thm]
+THEN `q' + &LENGTH P' - &LENGTH P' = q'` by fsa []
+THEN metis_tac [])
+
+THEN metis_tac [CHANGE_PC_INSTR_THM])
+
+THEN Cases_on `r` THEN fs [incr_pc_def]
+
+
+
+THEN rw [Once RTC_CASES2]
+
+THEN `exec_one (P' ++ P) (q' + &LENGTH P', stk, st) (q'' + &LENGTH P', stk', st')` by rw [exec_one_cases] THEN fsa [] THEN metis_tac [INT_ADD_COMM]);
+
+val EXECUTION_COMPOSE_THM = store_thm("EXECUTION_COMPOSE_THM",
+``!P P' stk st i' stk' st' i'' stk'' st''.exec P (0, stk, st) (i', stk', st') /\ (&LENGTH P <= i') /\ exec 
+P' (i' - &LENGTH P, stk', st') (i'', stk'', st'') ==> exec (P ++ P') (0, stk, st) (&LENGTH P + i'', stk'', st'')``,
+rw []
+
+THEN `(exec (P ++ P')) (0, stk, st) (i', stk', st')` by fsa [APPEND_TRACE_SAME_THM]
+
+THEN `(exec (P ++ P')) (incr_pc (i' - &LENGTH P,stk',st') (&LENGTH P)) (incr_pc (i'',stk'',st'') (&LENGTH P))` by fsa [APPEND_TRACE_SAME_2_THM]
+
+THEN fsa [incr_pc_def]
+
+THEN fsa [exec_def, INT_ADD_COMM]
+THEN metis_tac [RTC_TRANSITIVE, transitive_def]);
+
+
+
+
 val _ = export_theory ();
